theory/BitsOpMore3.thy
@@ -5,6 +5,39 @@ imports
 begin
 subsection \<open> u32_of_u8_list \<close>
 
+lemma ucast32_ucast8_and_255_eq [simp]: "ucast (((ucast (and v 255))::u8)) = and (v:: u32) 255"
+  apply (simp only: ucast_eq)
+(**r 
+word_of_int (uint (word_of_int (uint (and v 255)))) is
+
+(word_of_int (uint (and v 255)))::u8
+
+word_of_int (uint v_u8)  :: u64
+
+*)
+  apply (simp only: uint_word_of_int_eq word_and_def word_of_int_eq_iff)
+  apply (simp)
+  apply (simp add: bit_eq_iff)
+  apply (auto simp add: bit_simps)
+  subgoal for n
+    apply (cases n, simp_all)
+    subgoal for n1 apply (cases n1, simp_all)
+      subgoal for n2 apply (cases n2, simp_all)
+        subgoal for n3 apply (cases n3, simp_all)
+          subgoal for n4 apply (cases n4, simp_all)
+            subgoal for n5 apply (cases n5, simp_all)
+              subgoal for n6 apply (cases n6, simp_all)
+                subgoal for n6 apply (cases n6, simp_all)
+                  done
+                done
+              done
+            done
+          done
+        done
+      done
+    done
+  done
+
 lemma u32_shl_shr_same: "n \<le> 24 \<Longrightarrow> ((ucast (v::u8) ::u32) << n) >> n = (ucast (v::u8) ::u32)"
   apply (simp add: bit_eq_iff)
   apply (auto simp add: bit_simps)
@@ -32,13 +65,13 @@ lemma u32_shl_shr_outside: "n+8 \<le> m \<Longrightarrow> ((ucast (v::u8) ::u32)
   apply (auto simp add: bit_simps u8_ge_8_bit_false)
   done
 
-lemma [simp]: "(n::nat) \<le> 24 \<Longrightarrow> m \<le> n \<Longrightarrow> k < 32 \<Longrightarrow> n - m \<le> k \<Longrightarrow> k + m - n < 8 \<Longrightarrow> m + k < 32"
+lemma n_le_24_plus_lt_32: "(n::nat) \<le> 24 \<Longrightarrow> m \<le> n \<Longrightarrow> k < 32 \<Longrightarrow> n - m \<le> k \<Longrightarrow> k + m - n < 8 \<Longrightarrow> m + k < 32"
   by simp
 
 lemma u32_shl_shr_same_minus: "n \<le> 24 \<Longrightarrow> m \<le> n \<Longrightarrow>
   ((ucast (v::u8) ::u32) << n) >> m = ((ucast (v::u8) ::u32) << (n-m))"
   apply (simp add: bit_eq_iff)
-  apply (auto simp add: bit_simps u8_bit_true_ge_8)
+  apply (auto simp add: bit_simps u8_bit_true_ge_8 n_le_24_plus_lt_32)
   subgoal for k
     by (simp add: add.commute)
   subgoal for k
@@ -89,8 +122,7 @@ lemma u32_ucast_and_ucast_255_same: "(ucast (and (ucast (v::u8)) (255::u32)) ::u
   done
 
 
-
-lemma [simp]: "8 \<le> m \<Longrightarrow> (ucast (v::u8) ::u32) >> m = (0 ::u32)"
+lemma le_m_shr_0 : "8 \<le> m \<Longrightarrow> (ucast (v::u8) ::u32) >> m = (0 ::u32)"
   apply (simp add: bit_eq_iff)
   apply (auto simp add: bit_simps u8_ge_8_bit_false)
   done
@@ -100,20 +132,62 @@ lemma list_consists_4 : "length l = 4 \<Longrightarrow>
   by (smt (z3) add_2_eq_Suc' length_0_conv length_Suc_conv nth_Cons_0
       nth_Cons_Suc numeral_2_eq_2 numeral_3_eq_3 numeral_Bit0)
 
-lemma [simp]: "(Some v = u32_of_u8_list l) = (l = u8_list_of_u32 v)"
+lemma length_4_bit_eq: "(\<forall>n. bit (length l) n = bit (4::nat) n) \<Longrightarrow> length l = 4"
+  by (simp add: bit_eq_iff)
+
+lemma [simp]: "and (((v::u32) >> 24) << 24) 4278190080 = and v 4278190080"
+  apply (simp add: bit_eq_iff)
+  apply (auto simp add: bit_simps)
+  subgoal for n using bit_power_k_add_m_ge [of 24 8 n] by simp
+  subgoal for n using bit_power_k_add_m_ge [of 24 8 n] by simp
+  done
+
+lemma [simp]: "and (((v::u32) >> 16) << 16) 16711680 = and v 16711680"
+  apply (simp add: bit_eq_iff)
+  apply (auto simp add: bit_simps)
+  subgoal for n using bit_power_k_add_m_ge [of 16 8 n] by simp
+  subgoal for n using bit_power_k_add_m_ge [of 16 8 n] by simp
+  done
+
+lemma [simp]: "and (((v::u32) >> 8) << 8) 65280 = and v 65280"
+  apply (simp add: bit_eq_iff)
+  apply (auto simp add: bit_simps)
+  subgoal for n using bit_power_k_add_m_ge [of 8 8 n] by simp
+  subgoal for n using bit_power_k_add_m_ge [of 8 8 n] by simp
+  done
+
+lemma bit_255_not_lt_32 : "n < 32 \<Longrightarrow>
+  \<not> bit (4278190080::int) n \<Longrightarrow> \<not> bit (16711680::int) n \<Longrightarrow>
+  \<not> bit (65280::int) n \<Longrightarrow> bit (255::int) n"
+  using bit_power_k_add_m_lt [of n 24 8] apply simp
+  using bit_power_k_add_m_lt [of n 16 8] apply simp
+  using bit_power_k_add_m_lt [of n 8  8] apply simp
+  using bit_power_k_add_m_lt [of n 0  8] apply simp
+  apply blast
+  done
+
+lemma u32_of_u8_list_same: "(Some v = u32_of_u8_list l) = (l = u8_list_of_u32 v)"
   apply (unfold u32_of_u8_list_def u8_list_of_u32_def)
   apply (cases "length l \<noteq> 4", simp_all)
   subgoal by fastforce
   subgoal
     apply (rule iffI)
-    subgoal apply simp
+    subgoal
+      apply simp
+      apply (simp add: bit_eq_iff)
+      apply (auto simp add: bit_simps u32_shl_shr_same u32_shl_shr_outside le_m_shr_0
+          u32_shl_shr_same_minus u32_and_or_255_same u32_ucast_and_ucast_255_same)
+
+      subgoal using list_consists_4 length_4_bit_eq
+        by blast
+      done
 
     subgoal
       apply (simp add: bit_eq_iff)
       apply (simp add: bit_or_iff)
-      apply (auto simp add: bit_simps u32_shl_shr_same u32_shl_shr_outside
-          u32_shl_shr_same_minus u32_and_or_255_same u32_ucast_and_ucast_255_same)
-      subgoal using list_consists_4 
+      apply (auto simp add: bit_simps)
+      subgoal for n
+        using bit_255_not_lt_32 by blast
       done
     done
   done
